theories/Dot/fundamental.v
@@ -1,7 +1,8 @@
 From iris.proofmode Require Import tactics.
 From D Require Import swap_later_impl.
-From D.Dot Require Import unary_lr typing typeExtractionSem typing_unstamped.
-From D.Dot Require Import lr_lemma lr_lemmasDefs lr_lemma_nobinding lr_lemmasTSel.
+From D.Dot Require Import unary_lr typing typeExtractionSem typing_unstamped
+  lr_lemma lr_lemmasDefs lr_lemma_nobinding lr_lemmasTSel
+  astStamping typingStamping skeleton.
 
 Implicit Types (L T U: ty) (v: vl) (e: tm) (d: dm) (ds: dms) (Γ : ctx).
 
@@ -76,30 +77,28 @@ Section fundamental.
   Qed.
 
   Lemma fundamental_typed_upd Γ e T :
-    Γ ⊢ₜ e : T → allGs ∅ -∗ |==> Γ ⊨ e : T.
+    Γ ⊢ₜ e : T → allGs ∅ ==∗ Γ ⊨ e : T.
   Proof.
-    iIntros. iApply fundamental_typed => //. by iApply transfer_empty.
+    iIntros (HuT) "?". iApply (fundamental_typed HuT). by iApply transfer_empty.
   Qed.
-
 End fundamental.
 
 (** Adequacy of our logical relation: semantically well-typed terms are safe. *)
 
 Import dlang_adequacy.
 
-Theorem adequacy Σ `{HdlangG: dlangPreG Σ} `{SwapProp (iPropSI Σ)} e e' thp σ σ' T:
-  (forall `{!dlangG Σ} `{!SwapProp (iPropSI Σ)}, allGs ∅ ⊢ |==> [] ⊨ e : T) →
-  rtc erased_step ([e], σ) (thp, σ') → e' ∈ thp →
-  is_Some (to_val e') ∨ reducible e' σ'.
-Proof.
-  intros Hlog; eapply (adequacy _).
-  iIntros (??) "Hs"; iDestruct (Hlog with "Hs") as ">#H".
-  by iSpecialize ("H" $! ids with "[#//]"); rewrite hsubst_id.
-Qed.
-
 Definition safe e :=
   ∀ e' thp σ σ', rtc erased_step ([e], σ) (thp, σ') → e' ∈ thp →
     is_Some (to_val e') ∨ reducible e' σ'.
+
+Theorem adequacy Σ `{HdlangG: dlangPreG Σ} `{SwapProp (iPropSI Σ)} e T:
+  (∀ `{!dlangG Σ} `{!SwapProp (iPropSI Σ)}, allGs ∅ ⊢ |==> [] ⊨ e : T) →
+  safe e.
+Proof.
+  intros Hlog ?*; eapply (adequacy _).
+  iIntros (??) "Hs". iDestruct (Hlog with "Hs") as ">#Ht".
+  by iSpecialize ("Ht" $! ids with "[#// ]"); rewrite hsubst_id.
+Qed.
 
 (** Instead of still assuming semantic typing, here we should assume syntactic
     typing and use the fundamental lemma. But otherwise this follows the general
@@ -108,20 +107,16 @@ Definition safe e :=
 Corollary type_soundness_stamped e T `{!stampTable}:
   [] ⊢ₜ e : T → safe e.
 Proof.
-  intros HuT????; apply: (@adequacy dlangΣ _ _) => // *.
-  by iApply fundamental_typed_upd.
+  intros; apply: (@adequacy dlangΣ _ _)=>*. exact: fundamental_typed_upd.
 Qed.
-
-From D.Dot Require Import astStamping typingStamping skeleton.
 
 Lemma safe_same_skel e e_s:
   same_skel_tm e e_s → safe e_s → safe e.
 Proof.
-  rewrite /safe; intros Hst Hsafe ???? Hred Hin.
-  pose proof (simulation_skeleton_erased_steps Hst Hred Hin)
+  rewrite /safe; intros Hst Hsafe * Hred Hin.
+  destruct (simulation_skeleton_erased_steps Hst Hred Hin)
     as (e_s' & Hst_s & Hskel').
-  efeed pose proof Hsafe as [|];
-    [apply Hst_s|apply elem_of_list_here|left|right].
+  edestruct Hsafe; [apply Hst_s|apply elem_of_list_here|left|right].
   - destruct e_s', e'; naive_solver.
   - exact: same_skel_reducible.
 Qed.
@@ -133,6 +128,6 @@ Proof. move => [/unstamp_same_skel_tm Hs _] Hsafe. exact: safe_same_skel. Qed.
 Theorem type_soundness e T :
   [] u⊢ₜ e : T → safe e.
 Proof.
-  intros HuT. destruct (stamp_typed HuT ∅) as (e_s & g & HsT & ? & Hs).
+  intros (e_s & g & HsT & Hs)%stamp_typed.
   eapply (safe_stamp Hs), type_soundness_stamped, HsT.
 Qed.
